GenericModuleLib/MImplmn1.v
@@ -1,0 +1,368 @@
+(* %%%%%%%%%%%%%%%%%%%%%%%%%%%%%%%%%%%%%%%%%%%%%%%%%%%%%%%%%%%%%%%%% *) 
+(* Module with Certified Checking 
+   of the simplest module-interface.
+  
+   Last Update: Wed, 3 May 2017
+ %%%%%%%%%%%%%%%%%%%%%%%%%%%%%%%%%%%%%%%%%%%%%%%%%%%%%%%%%%%%%%%%%%% *) 
+
+Add LoadPath "../..".
+
+Require Import ConceptParams.AuxTactics.LibTactics.
+Require Import ConceptParams.AuxTactics.BasicTactics.
+
+Require Import ConceptParams.SetMapLib.List2Set.
+Require Import ConceptParams.SetMapLib.ListPair2FMap.
+
+Require Import ConceptParams.GenericModuleLib.MIntrfs1.
+
+Require Import Coq.Lists.List.
+Import ListNotations.
+Require Import Coq.Bool.Bool.
+
+Require Import Coq.Structures.Orders.
+Require Import Coq.Structures.Equalities.
+
+(* ***************************************************************** *)
+(** * Module-Implementation 1 
+
+      The Simplest Semantics of Modules *)
+
+(** Module-Implementation is well-defined with respect to
+    if
+    all names are different 
+    and all types are well-defined. *)
+(* ***************************************************************** *)
+(* ***************************************************************** *)
+
+(* ################################################################# *)
+(** ** Module Types defining Parameters *)
+(* ################################################################# *)
+
+Module Type DepData.  
+  (* contains types [t] and [ctx] *)
+  Include Data. 
+
+  (** Type of Local Context *)
+  Parameter ctx_local : Type.
+End DepData.
+
+Module Type DepDataOkDef (Import D : DepData) 
+       (Import MI : IntrfsBase).
+  (* element is ok on its own, 
+   * and it also corresponds to the interface *)
+  Parameter is_ok : ctx -> intrfs_map -> ctx_local -> 
+                    id -> t -> Prop.
+End DepDataOkDef.
+
+Module Type DepDataOkInterp (Import D : DepData)
+       (Import MI : IntrfsBase).
+  Parameter is_ok_b : ctx -> intrfs_map -> ctx_local -> 
+                      id -> t -> bool.
+End DepDataOkInterp.
+
+Module Type DepDataOkProp (Import D : DepData) 
+       (Import MI : IntrfsBase)
+       (Import DDef : DepDataOkDef D MI) (Import DInt : DepDataOkInterp D MI).
+
+  Axiom is_ok_b__sound : 
+    forall (c : ctx) (imap : MI.intrfs_map) (cl : ctx_local)
+           (nm : id) (x : t),
+      is_ok_b c imap cl nm x = true -> is_ok c imap cl nm x.
+
+  Axiom is_ok_b__complete : 
+    forall (c : ctx) (imap : MI.intrfs_map) (cl : ctx_local) 
+           (nm : id) (x : t),
+      is_ok c imap cl nm x -> is_ok_b c imap cl nm x = true.
+End DepDataOkProp.
+
+(* ################################################################# *)
+(** ** Shared Parameters of all building blocks *)
+(* ################################################################# *)
+
+Module Type ImplmnBase (Import MI : IntrfsBase).
+  (** Module of a corresponding interface (the data depends on) *)
+(*  Declare Module MI : IntrfsBase. *)
+
+  (* Terms Data *) 
+  Declare Module TmDT : DepData.
+  Definition tm := TmDT.t.
+
+  Definition implmn_ast := list (id * tm).
+  Definition implmn_map := IdLPM.id_map tm.
+End ImplmnBase.
+
+Module Type Implmn1Base (Import MI : IntrfsBase).
+  Include (ImplmnBase MI).
+
+  Definition ctx := TmDT.ctx.
+
+  Definition ctx_local := TmDT.ctx_local.
+  (** Initial local context *)
+  Parameter ctxl_init : ctx_local.
+  (** Update local context *)
+  Parameter upd_ctx_local : ctx_local -> ctx -> intrfs_map -> 
+                            id -> tm -> ctx_local.
+End Implmn1Base.
+
+(* ################################################################# *)
+(** ** Propositional Part *)
+(* ################################################################# *)
+
+Module MImplmn1Defs 
+       (Import MI : IntrfsBase)
+       (Import MIB : Implmn1Base MI) 
+       (Import TOkD : DepDataOkDef MIB.TmDT MI).
+
+  Definition process_dep_member
+             (c : ctx) (imap : intrfs_map)
+             (okAndCl : Prop * ctx_local) (def : id * tm) 
+  : Prop * ctx_local :=
+    match okAndCl with (ok_prop, cl) =>
+    match def with (nm, t) =>
+      let ok_prop' := 
+          (* check curr member in the local context *)
+          TOkD.is_ok c imap cl nm t  
+          (* and preserve previous members' part *)
+          /\ ok_prop in
+      (* update local context *)
+      let cl' := MIB.upd_ctx_local cl c imap nm t in
+      (ok_prop', cl')
+    end end.
+
+  Definition terms_ok' 
+             (c : ctx) (imap : intrfs_map) (cl : ctx_local)
+             (defs : list (id * tm)) : Prop * ctx_local :=
+    List.fold_left
+      (process_dep_member c imap)
+      defs
+      (True, cl).
+
+  Definition terms_ok 
+             (c : ctx) (imap : intrfs_map) 
+             (defs : list (id * tm)) : Prop :=
+    fst (terms_ok' c imap ctxl_init defs).
+
+
+  Definition implmn_ok 
+             (c : ctx) (imap : intrfs_map) 
+             (defs : list (id * tm)) : Prop :=
+    let nms := IdLPM.get_ids defs in
+    (** all names are distinct *)
+    List.NoDup nms
+    (** and all members are valid *)
+    /\ terms_ok c imap defs. 
+
+End MImplmn1Defs.
+
+(* ################################################################# *)
+(** ** Computable Part (static checker of the interpreter) *)
+(* ################################################################# *)
+
+Module MImplmn1Interp 
+       (Import MI : IntrfsBase)
+       (Import MIB : Implmn1Base MI) 
+       (Import TOkI : DepDataOkInterp MIB.TmDT MI).
+
+  
+  Definition process_dep_member_b 
+             (c : ctx) (imap : intrfs_map)
+             (okAndCl : bool * ctx_local) (def : id * tm) 
+  : bool * ctx_local :=
+    match okAndCl with 
+    | (true, cl) =>
+      match def with (nm, t) =>
+        let ok := TOkI.is_ok_b c imap cl nm t in
+        let cl' := MIB.upd_ctx_local cl c imap nm t in
+        (ok, cl')
+      end 
+    | (false, cl) => (false, cl)
+    end.
+
+  Definition terms_ok'_b 
+             (c : ctx) (imap : intrfs_map) (cl : ctx_local)
+             (defs : list (id * tm)) : bool * ctx_local :=
+    List.fold_left
+      (process_dep_member_b c imap)
+      defs
+      (true, cl).
+
+  Definition terms_ok_b 
+             (c : ctx) (imap : intrfs_map) 
+             (defs : list (id * tm)) : bool :=
+    fst (terms_ok'_b c imap ctxl_init defs).
+
+  Definition implmn_ok_b 
+             (c : ctx) (imap : intrfs_map) 
+             (defs : list (id * tm)) : bool :=
+    let nms := IdLPM.get_ids defs in
+    andb
+      (** all names are distinct *)
+      (IdLS.ids_are_unique nms)
+      (** and all types are valid *)
+      (terms_ok_b c imap defs).
+ 
+End MImplmn1Interp.
+
+(* ################################################################# *)
+(** ** Proofs of Correctness *)
+(* ################################################################# *)
+
+Module MImplmn1Props 
+       (Import MI : IntrfsBase)
+       (Import MIB : Implmn1Base MI) 
+       (Import TOkD : DepDataOkDef MIB.TmDT MI)
+       (Import TOkI : DepDataOkInterp MIB.TmDT MI)
+       (Import TOkP : DepDataOkProp MIB.TmDT MI TOkD TOkI)
+.
+  Module Import MID := MImplmn1Defs   MI MIB TOkD.
+  Module Import MII := MImplmn1Interp MI MIB TOkI.
+
+
+  Lemma process_dep_member_b_preserves_false :
+    forall (c : ctx) (imap : intrfs_map)
+           (ds : list (id * tm)) (cl : ctx_local),
+      fold_left (process_dep_member_b c imap) ds (false, cl) = (false, cl).
+  Proof.
+    intros c imap ds.
+    induction ds as [| [nm t] ds' IHds'];
+      intros cl.
+    - (* ds = nil *)
+      simpl. reflexivity.
+    - (* ds = (nm, t) :: ds' *)
+      simpl. apply IHds'.
+  Qed.
+
+  Lemma terms_ok'_b_cons_true :
+    forall (c : ctx) (imap : intrfs_map)
+           (ds : list (id * tm)) (cl : ctx_local)
+           (nm : id) (t : tm),
+      fst (terms_ok'_b c imap cl ((nm, t) :: ds)) = true ->
+      fst (terms_ok'_b c imap (upd_ctx_local cl c imap nm t) ds) = true.
+  Proof.
+    intros c imap ds.
+    unfold terms_ok'_b. simpl.
+    intros cl nm t H.
+    assert (Hok : is_ok_b c imap cl nm t = true).
+    { destruct (is_ok_b c imap cl nm t) eqn:Heq.
+      reflexivity.
+      destruct ds as [| d ds'].
+      + simpl in H. assumption.
+      + rewrite (process_dep_member_b_preserves_false c imap _ _) in H.
+        simpl in H. inversion H. }
+    rewrite Hok in H. assumption.
+  Qed.
+
+  Lemma terms_ok'_b_true__head_ok :
+    forall (c : ctx) (imap : intrfs_map)
+           (ds : list (id * tm)) (cl : ctx_local)
+           (nm : id) (t : tm),
+      fst (terms_ok'_b c imap cl ((nm, t) :: ds)) = true ->
+      is_ok_b c imap cl nm t = true.
+  Proof.
+    intros c imap ds cl nm t H.
+    unfold terms_ok'_b in H. simpl in H.
+    destruct (is_ok_b c imap cl nm t) eqn:Heq.
+    reflexivity.
+    rewrite (process_dep_member_b_preserves_false c imap _ _) in H.
+    simpl in H. assumption.
+  Qed.
+
+
+
+  Lemma terms_ok'__head_ok :
+    forall (c : ctx) (imap : intrfs_map)
+           (ds : list (id * tm)) (cl : ctx_local)
+           (nm : id) (t : tm),
+      fst (terms_ok' c imap cl ((nm, t) :: ds)) ->
+      is_ok c imap cl nm t.
+  Proof.
+    intros c imap ds cl nm t H.
+    unfold terms_ok' in H. simpl in H.
+    
+  Abort.
+
+  Lemma process_dep_member__any_prop :       
+    forall (c : ctx) (imap : intrfs_map)
+           (defs : list (id * tm)) (cl : ctx_local) (P P' : Prop),
+      P -> P' ->
+      fst (List.fold_left (process_dep_member c imap) defs (P, cl)) ->
+      fst (List.fold_left (process_dep_member c imap) defs (P', cl)).
+  Proof.
+    intros c imap ds.
+    induction ds as [| [nm t] ds' IHds'];
+      intros cl P P' HP HP' H.
+    - (* ds = nil *)
+      simpl. assumption.
+    - (* ds = (nm, t) :: ds' *)
+      simpl in *. 
+      apply IHds' with (P := is_ok c imap cl nm t /\ P).
+  Abort.
+
+    
+
+
+  Lemma terms_ok'_b__sound :
+    forall (c : ctx) (imap : intrfs_map)
+           (defs : list (id * tm)) (cl : ctx_local),
+      fst (terms_ok'_b c imap cl defs) = true ->
+      fst (terms_ok' c imap cl defs).
+  Proof.
+    intros c imap ds.
+    induction ds as [| [nm t] ds' IHds'];
+      intros cl H.
+    - constructor.
+    - (* ds = (nm, t) :: ds' *)
+      assert (H' := H).
+      apply terms_ok'_b_true__head_ok in H'.
+      unfold terms_ok'. simpl.
+      apply TOkP.is_ok_b__sound in H'.
+      assert (HTrue : is_ok c imap cl nm t /\ True <-> True).
+      { split; intros HT.
+        constructor.
+        split; assumption. }
+      unfold terms_ok' in IHds'.
+(*      rewrite -> HTrue.
+      
+      apply IHds'.
+      
+      unfold terms_ok'_b in H.
+      simpl in H.
+      specialize (IHds' 
+
+      apply terms_ok'_b_cons_true in H.
+  
+      unfold terms_ok'. simpl.
+      destruct d as [nm tm].
+*)
+  Abort.
+
+  Lemma terms_ok_b__sound :
+    forall (c : ctx) (imap : intrfs_map) (defs : list (id * tm)),
+      terms_ok_b c imap defs = true ->
+      terms_ok c imap defs.
+  Proof.
+    intros c imap ds.
+    induction ds as [| d ds' IHds'];
+      intros H.
+    - constructor.
+    - (* ds = d :: ds' *)
+      unfold terms_ok.
+
+  Abort.
+
+
+
+
+(* ----------------------------------------------------------------- *)
+(** *** Helper Props  *)
+(* ----------------------------------------------------------------- *)
+
+  Module Helper.
+
+  End Helper.
+
+
+End MImplmn1Props.
+
+
+
